c17lemmas.v
@@ -1,0 +1,90 @@
+Lemma sw_acy: acyclic sw.
+Proof.
+  destruct (mo_total_order_per_loc 0) as [spo _].
+  assert (sw⁺ ⊆ (`mo)^?%rel ⨾ rf).
+    intros x y swxy.
+    induction swxy.
+    destruct H as (x' & [<- xrel] & e & ers & y' & yrf & [-> yacq]).
+    esplit; esplit.
+    2: eauto.
+    destruct ers as [<-|[(x' & [<- xrel2] & moxe) _]].
+    left; auto.
+    auto.
+    destruct IHswxy1 as (e & moxe & rfy).
+    destruct IHswxy2 as (f & moyf & rfz).
+    destruct (rfy) as (eiw & yir & _).
+    destruct moyf as [<-|moyf].
+    
+    destruct (rfz) as (yiw & zir & _).
+    assert (yrmw: IsRMW y).
+      unfold IsRead in yir.
+      unfold IsWrite in yiw.
+      unfold IsRMW.
+      destruct (`y).
+      1-4: compute in yir, yiw; try discriminate yir; try discriminate yiw.
+      reflexivity.
+    lapply (rmw_atomic e y).
+    intros moey.
+    esplit; esplit.
+    2: apply rfz.
+    right.
+    destruct moey as (e' & f' & [moey _] & <- & <-).
+    destruct moxe as [->|(d' & e'' & moxe & <- & ff)].
+    repeat esplit; auto.
+    apply sig_ext in ff; subst e''.
+    repeat esplit.
+    apply spo with e'; auto.
+    esplit; esplit; eauto.
+    esplit; eauto.
+
+    destruct moyf as (e' & f' & moyf & <- & <-).
+    assert (yrmw: IsRMW (`e')).
+      destruct e' as [e' yiw].
+      unfold IsRead in yir.
+      unfold IsWrite in yiw.
+      unfold IsRMW.
+      simpl in *.
+      clear moyf.
+      destruct (`e').
+      1-4: compute in yir, yiw; try discriminate yir; try discriminate yiw.
+      reflexivity.
+    lapply (rmw_atomic e (`e')).
+    intros moey.
+    esplit; esplit.
+    2: apply rfz.
+    right.
+    destruct moey as (e'' & f'' & [moey _] & <- & ff).
+    apply sig_ext in ff; subst f''.
+    destruct moxe as [->|(d' & e''' & moxe & <- & ff)].
+    repeat esplit.
+    apply spo with e'; auto.
+    apply sig_ext in ff; subst e'''.
+    repeat esplit.
+    apply spo with e'; auto.
+    apply spo with e''; auto.
+    esplit; esplit; eauto.
+    esplit; eauto.
+  intros x rxx.
+  apply H in rxx.
+  destruct rxx as (e & moxe & rfx).
+  destruct moxe as [<-|(e' & f' & moey & <- & <-)].
+  apply rf_acy with x; constructor 1; auto.
+  assert (yrmw: IsRMW (`e')).
+    destruct e' as [e' yiw].
+    destruct rfx as [_ [yir _]].
+    unfold IsRead in yir.
+    unfold IsWrite in yiw.
+    unfold IsRMW.
+    simpl in *.
+    clear moey.
+    destruct (`e').
+    1-4: compute in yir, yiw; try discriminate yir; try discriminate yiw.
+    reflexivity.
+  lapply (rmw_atomic (`f') (`e')).
+  intros (e'' & f'' & [mofe _] & ee & ff).
+  apply sig_ext in ee; subst e''.
+  apply sig_ext in ff; subst f''.
+  apply spo with e'; apply spo with f'; auto.
+  esplit; esplit; eauto.
+  esplit; eauto.
+Qed.
