utils.v
@@ -1,0 +1,295 @@
+Lemma eq_dec_Op': forall o1 o2: Op', {o1 = o2} + {o1 <> o2}.
+Proof.
+  pose sig_ext.
+  pose f_equal.
+  decide equality.
+  decide equality.
+  all: assert (sumbool (`m = `m0) (`m <> `m0)).
+  1,3,5,7: decide equality.
+  destruct H.
+  left; auto. right; contradict n; auto.
+  destruct H0.
+  left; auto. right; contradict n; auto.
+  destruct H.
+  left; auto. right; contradict n; auto.
+  destruct H0.
+  left; auto. right; contradict n; auto.
+Qed.
+
+(*
+provide forall a, Acc r a - all elements accessible
+ - reverse map a to an inductive type l such that map(l) = a?
+ - induct on l, provide Acc r a in context C[l] to prove C[l] -> Acc r map(l)
+   - in base case b, provide C[b] -> Acc r map(b)
+     - eg there is no predecessor for map(b), all elems w/o predecessors reverse map to b
+   - in other case s with predecessors p, provide Acc r map(s) with C[s] and (C[p] -> Acc r map(p))
+     - if we didnt map(l) to a, Acc r a would not be rewritten to map(s) and map(p) in here
+     - then this would amount to proving C[p] from C[s] which is recursively proving a contradiction in C[b], but C[l] is sound remember?
+     - we prove C[p] from C[s] and then we have Acc r map(p) i.e. forall y, r y map(p) -> Acc r y
+     - forall y, r y map(s) -> forall y2, r y2 y -> eg if we can prove r y2 map(p), Acc r y2
+ - inductive type needs
+   - map(b) an object with fixed predecessors (eg none)
+   - map(s) can walk back a fixed # steps such that forall y, r y map(p) (eg 2)
+   - this is impossible - do we have to define the whole dag?
+     - Acc itself is like a dag
+ - Dont need to map l to a single a, map to a subset of a's by introducing a constraint in context
+   - prove forall a, C[l] -> Acc r a by induction, for some inductive l, C[l] expresses a constraint on a
+     - top level l must be chosen so C[top] is true for a
+     - top can be independent of a if C[top] is true for any a
+   - forall a, C[base] -> Acc r a
+     - forall a, C[base] -> forall y, r y a -> Acc r y
+     - C[base] constrains a to have no predecessors, forall y, r y a -> R(base) with R(base) -> False
+     - for List, base is []
+     - for Acc, base is any element _:Acc r a where forall y, r y a -> False
+   - (forall a, C[pred] -> Acc r a) -> forall a, C[succ] -> Acc r a:
+     - Given a constrained with C[succ], predecessors of a required to be constrained with C[pred]
+     - (forall b, (forall yp, r yp b -> R(pred)) -> Acc r b) ->
+       forall a,
+       (forall ys, r ys a -> R(succ)) ->
+       forall y,
+       r y a ->
+       Acc r y
+     - b = y, ys = y -> R(succ), (forall yp, r yp y -> R(pred)) -> Acc r y
+     - prove forall a y, r y a -> R(succ) -> forall yp, r yp y -> R(pred)
+     - given condition R(succ) on a y, r y a, and pred smaller than succ, prove R(pred) on yp, r yp y
+   - induction predecessors are chosen from the available structurally smaller types, in the successor calc
+   - So for R: forall a y (p: r y a) (l: inductive) -> Prop we need
+     - forall a y p, R a y p top
+     - forall a y p, R a y p base -> False
+     - forall a y p succ, R a y p succ ->
+         forall yp (pp: r yp y),
+         exists pred (_: Predecessor(succ,pred)),
+         R y yp pp pred
+     - R
+       - admits all a y in the biggest l
+       - provably admits no a y in the smallest l
+       - if it admits a y in l, it admits y yp in some inductive predecessor of l.
+   - suggests a scheme to iteratively restrict the a y that it admits
+     - in this case admitting a y in l means it must admit all transitive predecessor relations of y
+     - because r is acyclic, predecessor relations on predecessors of a do not need to support a
+       - exclude a with each step to meet the succ/pred condition
+     - because Op is finite, we have a list of all possible elements in r
+       - forall a _ _, R a _ _ list is inclusion of a in list
+       - full list is top
+       - empty list is base
+       - forall a _ _ succ, R a _ _ succ, the predecessor is succ excluding a
+     - need to define a list inductive type where forall a, excluding a is a predecessor
+       - Acc (fun x y => lenth(x) < length(y)) findom
+*)
+
+Lemma acy_wf: forall (r: relation Op), acyclic r -> well_founded r.
+Proof.
+  unfold well_founded, acyclic; intros r irr.
+  destruct events'_finite as [findom in_findom].
+  pose (sig_ext := sig_ext _ OP_WF).
+  (* pose (sig_ext2 := f_equal (@proj1_sig _ OP_WF)). *)
+  assert (findom_acc: Acc (fun x y => length(x) < length(y)) findom).
+  { clear in_findom.
+    constructor 1; induction findom.
+    2: constructor 1.
+    all: simpl in *; auto with *. }
+  assert (in_dom: forall o: Op, In (`o) findom).
+  { intros o; destruct o as [o' wf]. { destruct o'; red in wf; desf; auto. } }
+  intros.
+  assert (C: forall y, r⁺ y a -> In (` y) findom).
+  intros; apply in_dom.
+  clear in_dom in_findom; revert a C.
+  induction findom_acc; constructor 1; intros.
+  assert (H1t: r⁺ y a); auto with *.
+  specialize (C y H1t) as C_y.
+  pose (C_y2 := C_y); apply In_split in C_y2; destruct C_y2 as [l1 [l2 Heqsplit]]; subst x.
+  apply H0 with (l1 ++ l2).
+  rewrite !app_length; simpl; auto with *.
+  intros yp pp.
+  assert (`a <> `y).
+  intros ay; apply sig_ext in ay.
+  subst a.
+  apply irr with y.
+  auto with *.
+  generalize (C yp); rewrite !in_app_iff; simpl.
+  intros in_or; destruct in_or as [il1 | [ eq_a | il2 ]].
+  constructor 2 with y; auto.
+  auto.
+  apply sig_ext in eq_a; subst yp; apply irr in pp; auto with *.
+  auto.
+Qed.
+
+Lemma wf_t_invariant A (r: relation A):
+  well_founded r <-> well_founded r⁺.
+Proof.
+  split; intros WF; intros y.
+  induction y using (well_founded_induction WF).
+  constructor 1.
+  intros x rxy.
+  induction rxy.
+  auto.
+  apply IHrxy2; auto.
+  induction y using (well_founded_induction WF).
+  constructor 1.
+  intros x rxy.
+  apply H.
+  constructor 1.
+  auto.
+Qed.
+
+Lemma wf_acy A (r: relation A) (WF: well_founded r):
+  acyclic r.
+Proof.
+  apply wf_t_invariant in WF.
+  unfold acyclic, irreflexive, well_founded in *.
+  intros.
+  induction x using (well_founded_induction WF).
+  specialize (H0 x H H).
+  assumption.
+Qed.
+
+Lemma wf_not_infinite_descending A (r: relation A) (WF: well_founded r):
+  forall f, ~(forall n, r (f (S n)) (f n)).
+Proof.
+  unfold not; intros f.
+  remember (f 0) as x.
+  revert f Heqx.
+  specialize (WF x).
+  induction WF.
+  intros; subst x.
+  eapply H0 with (f := fun x => f (S x)).
+  eapply H1.
+  auto.
+  auto.
+  (* refine (
+      (fix rec n (a: Acc r (f n)) :=
+         match a
+         with
+           Acc_intro _ p =>
+             rec (S n) (p (f (S n)) (H n))
+         end) 0 WF). *)
+Qed.
+
+(*
+why is it so hard to prove that a prefix of a well-founded relation has a well founded inverse?
+because its false.
+ - we know r is well founded
+   - for all x, r is well-founded up to x
+   - meaning for all r y x we know r is well founded up to y
+   - which is the statement of inductibility
+     - a proposition P x is proved by induction on r if it can be proved assuming it's true for all
+       y prior to x in r.
+     - unrestricted fixpoints can prove anything so they must be constrained - fix p: ~sky(blue) := p
+       - If the fixpoint terminates, in the base case it does not call itself, so it
+         doesn't rely on itself for its own proof. Non-base cases are then proved incrementally upward.
+       - It terminates if it does not take any infinite path. Requiring fixpoints to descend a
+         well-founded relation is one way to achieve this.
+     - In coq, fixpoints are restricted by requiring them to descend in the structure of an inductive type
+       in order to invoke themselves
+       - for well-founded induction on x, we want to prove P x using proofs of P y for r y x. In the base
+         case there will be no such y.
+       - Our fixpoint will prove P x by descending some inductive Acc r x into Acc r y for all r y x
+         - fix proof_p x (a: Acc r x): P x :=
+             let prior_p y ryx := proof_p y (a y ryx) in _
+     - Our inductive Acc provides the minimal necessary access, and its type, forall y (r y x), forall z (r z y)
+       etc. essentially exhibits a proof that there are descending chains in r, and because it's an inductive,
+       a proof that these chains all terminate.
+       - fix Acc r x := forall y, r x y -> Acc r y
+   - How do you instantiate an inductive like Acc r x?
+     - By recursion on another inductive type, proving it in an assumption context C which is provable
+       at the top level:
+       - if x converts to (f i) and depends on i, induct on i to prove C i -> Acc r (f i)
+       - otherwise, induct on some i to prove forall x, C i x -> Acc r x
+     - At each step, the context assumption is available to prove Acc for current i, and to
+       induct we must provide proofs of the context assumptions for prior i from the current ones
+     - For Acc, to prove forall y, r y x -> Acc r y, we can manually construct Acc r y down to some
+       fixed depth, then we need inductive proofs of all predecessors.
+     - If induction gives access to (prior i) -> C (prior i) -> Acc r (f (prior i)),
+       - We can obtain Acc r y for all r y (f (prior i))
+       - We must be able to prove that after we costruct Acc r (f i) down to a fixed depth,
+         all Acc r y that we need to obtain will be for y that are r y (f (prior i))
+         - Similarly, in the base case with no (prior i), then there is no such y
+     - If induction gives access to (prior i) -> forall x, C (prior i) x Acc r x
+       - After constructing to fixed depth, forall Acc r y we need from induction we must
+         prove C (prior i) z for y = z or r y z
+       - And in the base case, with no (prior i), that there is no y
+     - The role of the context is to restrict the x in Acc r x so that in the base case there are no
+       predecessors, at the top level it doesnt restrict x at all, and at each step it restricts x
+       sufficiently that we can prove that the available Acc r y for C (prior i) y are sufficient to build Acc r x
+       - E.g. inducting on list l with context (r y x -> In y l) - complete in top case, empty in base case,
+         and restricting all our necessary y to be in l, we just need to prove that these y are also In y (prior l)
+*)
+
+Definition f_u x y :=
+  x <> 5 /\ (x < y \/ y = 5).
+
+Lemma wf_fu: well_founded f_u.
+Proof.
+  assert (forall x, x <> 5 -> Acc f_u x).
+  intros x xn5.
+  induction x using (well_founded_induction (Wf_nat.well_founded_ltof _ id)).
+  unfold Wf_nat.ltof, id in *.
+  constructor 1; intros y y0; destruct y0 as [yn5 [ylx|x5]].
+  apply H; assumption.
+  contradiction.
+  intros x.
+  constructor 1; intros y y0; destruct y0 as [yn5 _].
+  apply H; assumption.
+Qed.
+
+Lemma nwf_fu_inv: ~well_founded (f_u ⨾ ⦗f_u⁻¹ 5⦘)⁻¹.
+Proof.
+  intros wf; set (i := 6); specialize (wf i).
+  assert (i >= 6).
+  constructor 1.
+  induction wf.
+  eapply H1.
+  eexists.
+  split.
+  split.
+  auto with *.
+  left.
+  constructor 1.
+  split.
+  reflexivity.
+  split; auto with *.
+  auto with *.
+Qed.
+
+Lemma imm_trans: forall (r: relation Op), strict_partial_order r -> r ≡ (immediate r)⁺.
+Proof.
+  intros r [irr tra].
+  assert (acy: acyclic r).
+    assert (t: r⁺ ⊆ r).
+      intros x y rxy.
+      induction rxy.
+      auto.
+      eapply tra; eauto.
+    intros x rxx.
+    apply t in rxx.
+    eapply irr; eauto.
+  assert (ind := well_founded_induction (acy_wf r acy)).
+  eassert (ind_inv := well_founded_induction (acy_wf r⁻¹ ?[acy_inv])).
+  [acy_inv]: {
+    assert (H: forall x y, r⁻¹⁺ x y -> r⁺ y x).
+      intros x y rxy.
+      induction rxy.
+      constructor 1; assumption.
+      econstructor 2; eauto.
+    intros x rxx.
+    eapply acy; eapply (H x x); assumption.
+  }
+  split.
+  autounfold with unfolderDb.
+  intros x y; revert x.
+  induction y using ind.
+  intros x.
+  induction x using ind_inv.
+  destruct (classic (exists c, r x c /\ r c y)) as [[c [rxc rcy]]|n_imm].
+  constructor 2 with c.
+  apply H; auto.
+  apply H0; auto.
+  intros rxy; constructor 1; split; auto.
+  intros c rxc rcy; apply n_imm.
+  eexists; eauto.
+  autounfold with unfolderDb.
+  intros x y H.
+  induction H.
+  intuition.
+  apply tra with y; auto.
+Qed.
